theories/Shape.v
@@ -1,5 +1,11 @@
 From LinearCore Require
+  Fuel
+  Map
+  Reflect
   Term
+  .
+From LinearCore Require Import
+  Invert
   .
 
 
@@ -11,11 +17,119 @@ Variant shape : Set :=
 
 
 
-Inductive Shape : shape -> Term.term -> Prop :=
+Inductive ShapeOf : Term.term -> shape -> Prop :=
   | Ctr ctor
-      : Shape Resource (Term.Ctr ctor)
-  | App curried (curried_resource : Shape Resource curried) argument
-      : Shape Resource (Term.App curried argument)
+      : ShapeOf (Term.Ctr ctor) Resource
+  | App {curried} (curried_resource : ShapeOf curried Resource) argument
+      : ShapeOf (Term.App curried argument) Resource
   | Cas pattern body_if_match other_cases
-      : Shape Function (Term.Cas pattern body_if_match other_cases)
+      : ShapeOf (Term.Cas pattern body_if_match other_cases) Function
   .
+
+Lemma det {t s1} (S1 : ShapeOf t s1) {s2} (S2 : ShapeOf t s2)
+  : s1 = s2.
+Proof. generalize dependent s2. induction S1; intros; invert S2; reflexivity. Qed.
+
+
+
+Fixpoint shape_of t :=
+  match t with
+  | Term.Ctr _ => Some Resource
+  | Term.App curried argument =>
+      match shape_of curried with
+      | Some Resource => Some Resource
+      | _ => None
+      end
+  | Term.Cas _ _ _ => Some Function
+  | _ => None
+  end.
+
+Lemma shape_spec t
+  : Reflect.Option (ShapeOf t) (shape_of t).
+Proof.
+  induction t; cbn; try solve [constructor; intros s C; invert C].
+  - constructor. constructor.
+  - destruct IHt1. 2: { constructor. intros s C. invert C. apply N in curried_resource as []. }
+    destruct x; constructor. { constructor. exact Y. }
+    intros s C. invert C. assert (D := det Y curried_resource). discriminate D.
+  - constructor. constructor.
+Qed.
+
+
+
+Inductive ShapeOrRef context : Term.term -> shape -> Prop :=
+  | RCtr ctor
+      : ShapeOrRef context (Term.Ctr ctor) Resource
+  | RRef {name term} (F : Map.Find context name term)
+      {without_self} (R : Map.Remove name context without_self)
+      {shape} (S : ShapeOrRef without_self term shape)
+      : ShapeOrRef context (Term.Ref name) shape
+  | RApp {curried} (curried_resource : ShapeOf curried Resource) argument
+      : ShapeOrRef context (Term.App curried argument) Resource
+  | RCas pattern body_if_match other_cases
+      : ShapeOrRef context (Term.Cas pattern body_if_match other_cases) Function
+  .
+
+Lemma det_ref {c1 t s1} (S1 : ShapeOrRef c1 t s1) {c2}
+  (Ec : Map.Eq c1 c2) {s2} (S2 : ShapeOrRef c2 t s2)
+  : s1 = s2.
+Proof.
+  generalize dependent s2. generalize dependent c2. induction S1; intros; try solve [invert S2; reflexivity].
+  invert S2. eapply IHS1. 2: { apply Ec in F0. destruct (Map.find_det F F0). exact S. }
+  intros k v. destruct R as [D R]. cbn in R. rewrite R.
+  destruct R0 as [D0 R0]. cbn in R0. rewrite R0. cbn in Ec. rewrite Ec. reflexivity.
+Qed.
+
+Lemma eq_ref {c1 t s1} (S1 : ShapeOrRef c1 t s1) {c2}
+  (Ec : Map.Eq c1 c2) {s2} (Es : s1 = s2)
+  : ShapeOrRef c2 t s2.
+Proof.
+  generalize dependent s2. generalize dependent c2. induction S1; intros; subst; try solve [constructor].
+  - econstructor. { apply Ec. exact F. } 2: { exact S1. }
+    split. { eexists. apply Ec. exact F. } destruct R as [D R]. cbn in R.
+    intros k v. rewrite R. cbn in Ec. rewrite Ec. reflexivity.
+  - constructor. exact curried_resource.
+Qed.
+
+
+
+Fixpoint shape_or_ref fuel context t :=
+  match fuel with Fuel.Stop => Halt.OutOfFuel | Fuel.Continue fuel =>
+    match t with
+    | Term.Ctr _ => Halt.Return Resource
+    | Term.Ref name =>
+        match Map.find context name with None => Halt.Exit | Some term =>
+          shape_or_ref fuel (Map.remove name context) term
+        end
+    | Term.App curried argument =>
+        match shape_of curried with
+        | Some Resource => Halt.Return Resource
+        | _ => Halt.Exit
+        end
+    | Term.Cas _ _ _ => Halt.Return Function
+    | _ => Halt.Exit
+    end
+  end.
+
+Lemma shape_or_ref_spec fuel context t
+  : Reflect.Halt (ShapeOrRef context t) (shape_or_ref fuel context t).
+Proof.
+  generalize dependent t. generalize dependent context. induction fuel. { constructor. }
+  destruct t; cbn; try solve [constructor; intros s C; invert C].
+  - constructor. constructor.
+  - destruct (Map.find_spec context name). 2: { constructor. intros s C. invert C. apply N in F as []. }
+    destruct (IHfuel (Map.remove name context) x); constructor.
+    + econstructor. { exact Y. } 2: { exact Y0. } apply Map.remove_remove. eexists. exact Y.
+    + intros s C. invert C. destruct (Map.find_det Y F). eapply N. eapply eq_ref. { exact S. } 2: { reflexivity. }
+      intros k v. destruct R as [D R]. cbn in R. rewrite R. symmetry. apply Map.remove_if_present_remove.
+  - destruct (shape_spec t1). 2: { constructor. intros s C. invert C. apply N in curried_resource as []. }
+    destruct x; constructor. { constructor. exact Y. }
+    intros s C. invert C. assert (D := det Y curried_resource). discriminate D.
+  - constructor. constructor.
+Qed.
+
+
+
+Lemma or_ref {t s} (S : ShapeOf t s) context
+  : ShapeOrRef context t s.
+Proof. generalize dependent context. induction S; intros. { constructor. } { constructor. exact S. } constructor. Qed.
