theories/SmallStep.v
@@ -28,6 +28,9 @@ Inductive Step (context : Context.context) : Term.term -> Context.context -> Ter
       {context_updated_in_place} (update
         : Map.Add self stepped updated_context_without_self context_updated_in_place)
       : Step context (Term.Ref self) context_updated_in_place (Term.Ref self)
+  | ApF {function updated_context updated_function}
+      (reduce_function : Step context function updated_context updated_function) argument
+      : Step context (Term.App function argument) updated_context (Term.App updated_function argument)
   | ApM
       {pattern} (compatible_names : Match.Compatible context pattern)
       {scrutinee body_if_match other_cases} (unshadowed
@@ -52,7 +55,7 @@ Inductive Step (context : Context.context) : Term.term -> Context.context -> Ter
       {scrutinee body_if_match other_cases} (unshadowed
         : Unshadow.Unshadowed $ Term.App (Term.Cas pattern body_if_match other_cases) scrutinee)
       (no_match : forall context_with_matches (M : Match.Pattern context pattern scrutinee context_with_matches), False)
-      {shape} (scrutinee_reduced : Shape.Shape shape scrutinee)
+      {shape} (scrutinee_reduced : Shape.ShapeOrRef context scrutinee shape)
       {unchanged_context} (context_unchanged : Map.Eq context unchanged_context)
       : Step context
         (Term.App (Term.Cas pattern body_if_match other_cases) scrutinee) unchanged_context
@@ -70,13 +73,75 @@ Arguments Step context term updated_context updated_term.
 
 
 
+Lemma eq
+  {c1 t1 c1' t1'} (S1 : Step c1 t1 c1' t1')
+  {c2} (Ec : Map.Eq c1 c2)
+  {t2} (Et : t1 = t2)
+  {c2'} (Ec' : Map.Eq c1' c2')
+  {t2'} (Et' : t1' = t2')
+  : Step c2 t2 c2' t2'.
+Proof.
+  subst. rename t2 into t. rename t2' into t'. generalize dependent c2'. generalize dependent c2.
+  induction S1; intros.
+  - apply Mov. { apply Ec. exact lookup. } destruct no_contraction as [I R]. split.
+    + eapply Map.in_eq. { apply Map.eq_sym. exact Ec. } eexists. exact lookup.
+    + cbn in *. intros x y. rewrite <- Ec'. rewrite <- Ec. apply R.
+  - eapply Ref.
+    + apply Ec. exact lookup.
+    + destruct remove_self_from_context as [I R]. split.
+      * eapply Map.in_eq. { apply Map.eq_sym. exact Ec. } exact I.
+      * cbn in *. intros x y. rewrite R. rewrite Ec. reflexivity.
+    + exact S1.
+    + exact not_overwriting_self.
+    + cbn in *. intros x y. rewrite <- Ec'. apply update.
+  - apply ApF. apply IHS1. { exact Ec. } exact Ec'.
+  - apply ApM.
+    + eapply Match.compatible_eq; try reflexivity; eassumption.
+    + exact unshadowed.
+    + eapply Match.pattern_eq; try reflexivity; eassumption.
+  - apply ApS.
+    + eapply Match.compatible_eq; try reflexivity; eassumption.
+    + exact unshadowed.
+    + intros. eapply no_match. eapply Match.pattern_eq; try reflexivity;
+      try eassumption. { apply Map.eq_sym. eassumption. } apply Map.eq_refl.
+    + apply IHS1; eassumption.
+  - eapply ApN.
+    + eapply Match.compatible_eq; try reflexivity; eassumption.
+    + exact unshadowed.
+    + intros. eapply no_match. eapply Match.pattern_eq; try reflexivity;
+      try eassumption. { apply Map.eq_sym. eassumption. } apply Map.eq_refl.
+    + eapply Shape.eq_ref. { exact scrutinee_reduced. } { exact Ec. } reflexivity.
+    + eapply Map.eq_trans. { apply Map.eq_sym. exact Ec. }
+      eapply Map.eq_trans. { exact context_unchanged. } exact Ec'.
+  - eapply ApR.
+    + destruct not_yet_safe_to_match as [N | N]; [left | right]; intro C; apply N. 2: { exact C. }
+      eapply Match.compatible_eq. 3: { reflexivity. } { exact C. } apply Map.eq_sym. exact Ec.
+    + eapply Map.domain_eq. { exact D. } { exact Ec. } apply Map.eq_refl.
+    + exact rename.
+    + eapply Map.eq_trans. { apply Map.eq_sym. exact Ec. } eapply Map.eq_trans. { exact context_unchanged. } exact Ec'.
+Qed.
+
+
+
 Theorem shapes_cant_step
-  {shape term} (shaped : Shape.Shape shape term)
+  {term shape} (shaped : Shape.ShapeOf term shape)
   {context updated_context updated_term} (step : Step context term updated_context updated_term)
   : False.
 Proof.
   generalize dependent updated_term. generalize dependent updated_context. generalize dependent context.
-  induction shaped; intros; invert step; invert shaped.
+  induction shaped; intros; invert step; invert shaped. { invert reduce_function. } apply IHshaped in reduce_function as [].
+Qed.
+
+Theorem shape_or_ref_cant_step
+  {context term shape} (shaped : Shape.ShapeOrRef context term shape)
+  {updated_context updated_term} (step : Step context term updated_context updated_term)
+  : False.
+Proof.
+  generalize dependent updated_term. generalize dependent updated_context.
+  induction shaped; intros; try solve [invert step]. 2: { invert step; try solve [invert curried_resource].
+    eapply shapes_cant_step in curried_resource as []. exact reduce_function. }
+  invert step. destruct (Map.find_det F lookup). assert (Ew := Map.remove_det remove_self_from_context eq_refl (Map.eq_refl _) R).
+  eapply IHshaped. eapply eq. { exact step_in_context. } { exact Ew. } { reflexivity. } { apply Map.eq_refl. } reflexivity.
 Qed.
 
 
@@ -97,6 +162,13 @@ Proof.
     specialize (IHS1 _ RD). apply Ec in lookup0. destruct (Map.find_det lookup lookup0).
     specialize (IHS1 _ _ step_in_context) as [Eu <-]. eapply Map.add_det; try reflexivity; eassumption.
   - invert S2.
+    + specialize (IHS1 _ Ec _ _ reduce_function) as [E ->]. split. { exact E. } reflexivity.
+    + eapply shapes_cant_step in S1 as []. constructor.
+    + eapply shapes_cant_step in S1 as []. constructor.
+    + eapply shapes_cant_step in S1 as []. constructor.
+    + eapply shapes_cant_step in S1 as []. constructor.
+  - invert S2.
+    + eapply shapes_cant_step in reduce_function as []. constructor.
     + split. 2: { reflexivity. } eapply Match.pattern_det; try reflexivity; eassumption.
     + contradiction (no_match context_with_matches).
       eapply Match.pattern_eq; try reflexivity; try eassumption; apply Map.eq_refl.
@@ -105,22 +177,27 @@ Proof.
     + destruct not_yet_safe_to_match as [N | N]. 2: { apply N in unshadowed as []. }
       contradiction N. eapply Match.compatible_eq; try reflexivity; eassumption.
   - invert S2.
+    + eapply shapes_cant_step in reduce_function as []. constructor.
     + contradiction (no_match c2'). eapply Match.pattern_eq; try reflexivity; try eassumption. 2: { apply Map.eq_refl. }
       apply Map.eq_sym. exact Ec.
     + edestruct IHS1 as [Ec' E]. { exact Ec. } { exact reduce_scrutinee. } subst reduced_scrutinee0.
       split. { exact Ec'. } reflexivity.
-    + eapply shapes_cant_step in scrutinee_reduced as []. eassumption.
+    + eapply shape_or_ref_cant_step in scrutinee_reduced as [].
+      eapply eq. { exact S1. } { exact Ec. } { reflexivity. } { apply Map.eq_refl. } reflexivity.
     + destruct not_yet_safe_to_match as [N | N]. 2: { apply N in unshadowed as []. }
       contradiction N. eapply Match.compatible_eq; try reflexivity; eassumption.
   - invert S2.
+    + eapply shapes_cant_step in reduce_function as []. constructor.
     + contradiction (no_match c2'). eapply Match.pattern_eq; try reflexivity; try eassumption. 2: { apply Map.eq_refl. }
       apply Map.eq_sym. exact Ec.
-    + eapply shapes_cant_step in scrutinee_reduced as []. eassumption.
+    + eapply shape_or_ref_cant_step in scrutinee_reduced as [].
+      eapply eq. { exact reduce_scrutinee. } { apply Map.eq_sym. exact Ec. } { reflexivity. } { apply Map.eq_refl. } reflexivity.
     + split. 2: { reflexivity. } eapply Map.eq_trans. { apply Map.eq_sym. exact context_unchanged. }
       eapply Map.eq_trans. { exact Ec. } exact context_unchanged0.
     + destruct not_yet_safe_to_match as [N | N]. 2: { apply N in unshadowed as []. }
       contradiction N. eapply Match.compatible_eq; try reflexivity; eassumption.
   - invert S2.
+    + eapply shapes_cant_step in reduce_function as []. constructor.
     + destruct not_yet_safe_to_match as [N | N]. 2: { apply N in unshadowed as []. }
       contradiction N. eapply Match.compatible_eq; try reflexivity; try eassumption. apply Map.eq_sym. assumption.
     + destruct not_yet_safe_to_match as [N | N]. 2: { apply N in unshadowed as []. }
@@ -136,55 +213,6 @@ Qed.
 
 
 
-Lemma eq
-  {c1 t1 c1' t1'} (S1 : Step c1 t1 c1' t1')
-  {c2} (Ec : Map.Eq c1 c2)
-  {t2} (Et : t1 = t2)
-  {c2'} (Ec' : Map.Eq c1' c2')
-  {t2'} (Et' : t1' = t2')
-  : Step c2 t2 c2' t2'.
-Proof.
-  subst. rename t2 into t. rename t2' into t'. generalize dependent c2'. generalize dependent c2.
-  induction S1; intros.
-  - constructor. { apply Ec. exact lookup. } destruct no_contraction as [I R]. split.
-    + eapply Map.in_eq. { apply Map.eq_sym. exact Ec. } eexists. exact lookup.
-    + cbn in *. intros x y. rewrite <- Ec'. rewrite <- Ec. apply R.
-  - econstructor.
-    + apply Ec. exact lookup.
-    + destruct remove_self_from_context as [I R]. split.
-      * eapply Map.in_eq. { apply Map.eq_sym. exact Ec. } exact I.
-      * cbn in *. intros x y. rewrite R. rewrite Ec. reflexivity.
-    + exact S1.
-    + exact not_overwriting_self.
-    + cbn in *. intros x y. rewrite <- Ec'. apply update.
-  - constructor.
-    + eapply Match.compatible_eq; try reflexivity; eassumption.
-    + exact unshadowed.
-    + eapply Match.pattern_eq; try reflexivity; eassumption.
-  - constructor.
-    + eapply Match.compatible_eq; try reflexivity; eassumption.
-    + exact unshadowed.
-    + intros. eapply no_match. eapply Match.pattern_eq; try reflexivity;
-      try eassumption. { apply Map.eq_sym. eassumption. } apply Map.eq_refl.
-    + apply IHS1; eassumption.
-  - econstructor.
-    + eapply Match.compatible_eq; try reflexivity; eassumption.
-    + exact unshadowed.
-    + intros. eapply no_match. eapply Match.pattern_eq; try reflexivity;
-      try eassumption. { apply Map.eq_sym. eassumption. } apply Map.eq_refl.
-    + apply scrutinee_reduced.
-    + eapply Map.eq_trans. { apply Map.eq_sym. exact Ec. }
-      eapply Map.eq_trans. { exact context_unchanged. } exact Ec'.
-  - econstructor.
-    + destruct not_yet_safe_to_match as [N | N]; [left | right]; intro C; apply N. 2: { exact C. }
-      eapply Match.compatible_eq. 3: { reflexivity. } { exact C. } apply Map.eq_sym. exact Ec.
-    + eapply Map.domain_eq. { exact D. } { exact Ec. } apply Map.eq_refl.
-    + exact rename.
-    + eapply Map.eq_trans. { apply Map.eq_sym. exact Ec. } eapply Map.eq_trans. { exact context_unchanged. } exact Ec'.
-Qed.
-
-
-
 Theorem unshadowed_invariant {c t c' t'} (S : Step c t c' t')
   (Ut : Unshadow.Unshadowed t) (Uc : Map.ForAll (fun _ => Unshadow.Unshadowed) c)
   : Unshadow.Unshadowed t' /\ Map.ForAll (fun _ => Unshadow.Unshadowed) c'.
@@ -194,10 +222,13 @@ Proof.
   - split. { constructor. } intros k v F. destruct IHS as [U FA]. { eapply Uc. exact lookup. }
     + intros k' v' F'. apply remove_self_from_context in F' as [N' F']. eapply Uc. exact F'.
     + apply update in F as [[-> ->] | F]. { exact U. } eapply FA. exact F.
-  - cbn. invert unshadowed. invert Ut. invert Uf. invert Uf0. split. { exact Ub. } intros.
+  - invert Ut. specialize (IHS Uf Uc) as [IHt IHc]. split. { constructor. { exact IHt. } { exact Ua. } Abort.
+(*
+  - invert unshadowed. invert Ut. invert Uf. invert Uf0. split. { exact Ub. } intros.
     eapply Match.unshadow_pattern. { exact Ua. } { exact Uc. } { exact matched. } exact F.
   - invert unshadowed. invert Ut. specialize (IHS Ua Uc) as [IHt IHc]. split.
     + constructor; try eassumption; intros. { eapply disj_f_a0. { exact Bf. } Abort.
+ *)
 (* So, no, this is not worth enforcing. In other words, why have laziness if we're spending compute
  * renaming terms that we might never use? On the other hand, it costs compute to *check* and/or unshadow at every match.
  * TODO: maybe profile this? *)
