theories/SmallStepFunction.v
@@ -45,17 +45,86 @@ Fixpoint step (fuel : Fuel.fuel) (context : Context.context) (term : Term.term) 
           | other => other
           end
         end
-    | Term.App (Term.Cas pattern body_if_match other_cases) scrutinee =>
-        if andb (Match.compatible context pattern) (Unshadow.unshadowed term) then
-          Halt.Exit (* TODO *)
-        else
-          match Unshadow.unshadow_reserve (Map.domain context) term with
-          | None => Halt.Exit
-          | Some renamed => Halt.Return (context, renamed)
-          end
+    | Term.App function argument =>
+        match step fuel context function with
+        | Halt.OutOfFuel => Halt.OutOfFuel
+        | Halt.Return (updated_context, updated_function) =>
+            Halt.Return (updated_context, Term.App updated_function argument)
+        | Halt.Exit =>
+            match function with
+            | Term.Cas pattern body_if_match other_cases =>
+                if andb (Match.compatible context pattern) (Unshadow.unshadowed term) then
+                  match pattern with
+                  | Pattern.Nam name => Halt.Return (Map.overriding_add name argument context, body_if_match)
+                  | Pattern.Pat move_or_reference =>
+                      match Shape.shape_or_ref fuel context argument with
+                      | Halt.OutOfFuel => Halt.OutOfFuel
+                      | Halt.Return _ =>
+                          match Match.move_or_reference context move_or_reference argument with
+                          | None => Halt.Return (context, Term.App other_cases argument)
+                          | Some context_with_matches => Halt.Return (context_with_matches, body_if_match)
+                          end
+                      | Halt.Exit =>
+                          match step fuel context argument with
+                          | Halt.OutOfFuel => Halt.OutOfFuel
+                          | Halt.Exit => Halt.Exit
+                          | Halt.Return (updated_context, reduced_scrutinee) =>
+                              Halt.Return (updated_context, Term.App (Term.Cas pattern body_if_match other_cases) reduced_scrutinee)
+                          end
+                      end
+                  end
+                else
+                  match Unshadow.unshadow_reserve (Map.domain context) term with
+                  | None => Halt.Exit
+                  | Some renamed => Halt.Return (context, renamed)
+                  end
+            | _ => Halt.Exit
+            end
+        end
     | _ => Halt.Exit
     end
   end.
+
+
+
+Lemma step_app fuel context function argument
+  : step (Fuel.Continue fuel) context (Term.App function argument) =
+    match step fuel context function with
+    | Halt.OutOfFuel => Halt.OutOfFuel
+    | Halt.Return (updated_context, updated_function) =>
+        Halt.Return (updated_context, Term.App updated_function argument)
+    | Halt.Exit =>
+        match function with
+        | Term.Cas pattern body_if_match other_cases =>
+            if andb (Match.compatible context pattern) (Unshadow.unshadowed $ Term.App function argument) then
+              match pattern with
+              | Pattern.Nam name => Halt.Return (Map.overriding_add name argument context, body_if_match)
+              | Pattern.Pat move_or_reference =>
+                  match Shape.shape_or_ref fuel context argument with
+                  | Halt.OutOfFuel => Halt.OutOfFuel
+                  | Halt.Return _ =>
+                      match Match.move_or_reference context move_or_reference argument with
+                      | None => Halt.Return (context, Term.App other_cases argument)
+                      | Some context_with_matches => Halt.Return (context_with_matches, body_if_match)
+                      end
+                  | Halt.Exit =>
+                      match step fuel context argument with
+                      | Halt.OutOfFuel => Halt.OutOfFuel
+                      | Halt.Exit => Halt.Exit
+                      | Halt.Return (updated_context, reduced_scrutinee) =>
+                          Halt.Return (updated_context, Term.App (Term.Cas pattern body_if_match other_cases) reduced_scrutinee)
+                      end
+                  end
+              end
+            else
+              match Unshadow.unshadow_reserve (Map.domain context) $ Term.App function argument with
+              | None => Halt.Exit
+              | Some renamed => Halt.Return (context, renamed)
+              end
+        | _ => Halt.Exit
+        end
+    end.
+Proof. reflexivity. Qed.
 
 
 
@@ -63,11 +132,11 @@ Theorem spec fuel context term
   : Reflect.Halt (fun pair => SmallStep.Step context term (fst pair) (snd pair)) (step fuel context term).
 Proof.
   generalize dependent term. generalize dependent context. induction fuel. { constructor. }
-  destruct term; try solve [constructor; intros [updated_context updated_term] S; cbn in *; invert S].
-  - cbn in *. destruct (Map.find_spec context name); constructor; cbn in *.
+  destruct term; try solve [constructor; intros [updated_context updated_term] S; invert S].
+  - cbn. destruct (Map.find_spec context name); constructor; cbn in *.
     + constructor. { exact Y. } apply Map.remove_remove. eexists. exact Y.
     + intros [updated_context updated_term] S; cbn in *. invert S. apply N in lookup as [].
-  - cbn in *. destruct (Map.find_spec context name). 2: {
+  - cbn. destruct (Map.find_spec context name). 2: {
       constructor. intros [m t] C; cbn in *. invert C. apply N in lookup as []. }
     destruct (IHfuel (Map.remove name context) x). 3: { constructor. } 2: {
       constructor. intros [m t] C; cbn in *. invert C. eapply (N (_, _)). eapply SmallStep.eq.
@@ -88,9 +157,11 @@ Proof.
     cbn. econstructor. { exact Y. } { apply Map.remove_remove. eexists. exact Y. } { exact Y0. }
     + intros [y F]. apply N in F as [].
     + apply Map.add_overriding. intros v F. apply N in F as [].
-  - unfold step. unfold VerbosePrint.format. unfold VerbosePrint.print.
-    destruct term1 as [| | | | | pattern body_if_match other_cases];
-    try solve [constructor; intros [m t] C; invert C]. destruct andb eqn:E. 2: {
+  - rewrite step_app. destruct (IHfuel context term1) as [[updated_context updated_function] | |]. 3: { constructor. } {
+      constructor. cbn in *. apply SmallStep.ApF. exact Y. }
+    destruct term1 as [| | | | | pattern body_if_match other_cases]; try solve [
+      constructor; intros [m t] C; invert C; cbn in *; apply (N (_, _)) in reduce_function as []].
+    destruct andb eqn:E. 2: {
       apply Bool.andb_false_iff in E. destruct Unshadow.unshadow_reserve eqn:Eu; constructor.
       * cbn. eapply SmallStep.ApR. 3: { exact Eu. } 2: { apply Map.domain_domain. } 2: { apply Map.eq_refl. }
         destruct E as [E | E]; [left | right]; intro C.
@@ -98,9 +169,28 @@ Proof.
         -- apply Unshadow.unshadowed_iff in C. rewrite E in C. discriminate C.
       * intros [c' t'] C. simpl fst in *. simpl snd in *. invert C; try solve [destruct E as [E | E]; [
           apply Match.compatible_iff in compatible_names; rewrite E in compatible_names; discriminate compatible_names |
-          apply Unshadow.unshadowed_iff in unshadowed; rewrite E in unshadowed; discriminate unshadowed]].
+          apply Unshadow.unshadowed_iff in unshadowed; rewrite E in unshadowed; discriminate unshadowed]]. {
+          apply (N (_, _)) in reduce_function as []. }
         assert (Ed : Map.Eq (Map.domain context) context_domain). {
           eapply Map.domain_det. { apply Map.domain_domain. } 2: { exact D. } apply Map.eq_refl. }
         destruct (Unshadow.det_reserve Ed (@eq_refl _ $ Term.App (Term.Cas pattern body_if_match other_cases) term2)).
         rewrite Eu in rename. discriminate rename. }
-Abort.
+    apply Bool.andb_true_iff in E as [MC US]. apply Match.compatible_iff in MC. apply Unshadow.unshadowed_iff in US.
+    destruct pattern. { constructor. cbn. apply SmallStep.ApM; try assumption. invert MC.
+      constructor. { assumption. } apply Map.add_overriding. intros v F. contradiction N0. eexists. exact F. }
+    destruct (Shape.shape_or_ref_spec fuel context term2). 3: { constructor. }
+    + destruct (Match.move_or_reference_spec context move_or_reference term2); constructor; cbn.
+      * apply SmallStep.ApM. { exact MC. } { exact US. } constructor. exact Y0.
+      * eapply SmallStep.ApN. { exact MC. } { exact US. } 2: { exact Y. } 2: { apply Map.eq_refl. }
+        intros ? P. invert P. apply N0 in move_or_reference_matched as [].
+    + destruct (IHfuel context term2) as [[updated_context reduced_scrutinee] | |]; constructor.
+      * cbn in *. apply SmallStep.ApS. { exact MC. } { exact US. } 2: { exact Y. } intros ? P. invert P.
+        apply Match.move_or_reference_shape_or_ref in move_or_reference_matched as SR. apply N0 in SR as [].
+      * intros [c t] C. cbn in *. invert C.
+        -- apply (N (_, _)) in reduce_function as [].
+        -- invert matched. apply Match.move_or_reference_shape_or_ref in move_or_reference_matched.
+           apply N0 in move_or_reference_matched as [].
+        -- apply (N1 (_, _)) in reduce_scrutinee as [].
+        -- apply N0 in scrutinee_reduced as [].
+        -- destruct not_yet_safe_to_match as [NS | NS]; apply NS. { exact MC. } exact US.
+Qed.
